## Differentiation

$$
\begin{split}
(c)^{'} &= 0 \\
(kx)^{'} = k &\:,\: (ku)^{'} = ku^{'} \\
(x^n)^{'} = nx^{n-1} &\:,\: (u^n)^{'} = u^{'}nu^{n-1} \\\\
(uv)^{'} &= u^{'}v + v^{'}u \\
\left(\frac{u}{v}\right)^{'} &= \frac{u^{'}v - v^{'}u}{v^2} \\
\left(\frac{1}{x}\right)^{'} = -\frac{1}{x^2} &\:,\: \left(\frac{1}{u}\right)^{'} = \frac{u^{'}}{u^2} \\
\\
(\sqrt{x})^{'} = \frac{1}{2\sqrt{x}} &\:,\: (\sqrt{u})^{'} = \frac{u^{'}}{2\sqrt{u}} \\
\\
(\sin x)^{'} = \cos x &\:,\: (\sin u)^{'} = u^{'} \cos u \\
(\cos x)^{'} = - \sin x &\:,\: (\cos u)^{'} = - u^{'} \sin u  \\
\\
(e^x)^{'} = e^x &\:,\: (e^u)^{'} = u^{'} e^u \\
(a^x)^{'} = a^x \ln a &\:,\: (a^u)^{'} = u^{'}a^u \ln a \\
(\ln x)^{'} = \frac{1}{x} &\:,\: (\ln u)^{'} = \frac{u^{'}}{u} \\
(\log _ax)^{'} = \frac{1}{x\ln a} &\:,\: (\log _au)^{'} = \frac{u^{'}}{u\ln a} \\
\\
(u \pm v)^{'} &= u^{'} \pm v^{'} \\
(u_1 \pm \ldots \pm u_n)^{'} &= u_1^{'} \pm \ldots \pm u_n^{'} \\
y = y[u(x)] & \Rightarrow y^{'}(x) = y^{'}(u)u^{'}(x) \\
\left(\frac{ax+b}{cx+d}\right)^{'} &= \frac{\begin{vmatrix} a & b \\ c & d \end{vmatrix}}{(cx+d)^2} \\
\end{split}
$$

## Integral

$$
\begin{split}
\int dx = x  &\:,\: \int du = u  \\
\int x^{\alpha} dx = \frac{x^{\alpha +1}}{\alpha +1}  &\:,\: \int u^{\alpha} du = \frac{u^{\alpha +1}}{\alpha +1}  \\
\\
\int a^x dx = \frac{a^x}{\ln a} &\:,\: \int a^u dx = \frac{a^u}{\ln a} \\
\int \frac{dx}{x} = \ln |x| &\:,\: \int \frac{du}{u} = \ln |u| \\
\\
\int e^x dx = e^x &\:,\: \int e^u du = e^u  \\
\int e^{kx} dx &= \frac{e^kx}{k} \\
\\
\int \cos x dc = \sin x  &\:,\: \int \cos udu = \sin u \\
\int \sin xdx = - \cos x &\:,\: \int \sin udu = - \cos u  \\
\int \cos (ax+b)dx &= \frac{1}{a} \sin (ax+b) \\
\int \sin (ax+b) dx &= -\frac{1}{a} \cos (ax+b) \\
\\
\int (ax+b)^{\alpha} &= \frac{1}{a} \frac{(ax+b)^{\alpha +1}}{\alpha +1}  \\
\end{split}
$$

!!! warning
    Do not miss $+C$!

## Root of trigonometric

$$
\begin{split}
\sin u = 0 & \Rightarrow u =k \pi \\
\sin u = 1 & \Rightarrow u = \frac{\pi}{2} + k2\pi \\
\sin u = -1 & \Rightarrow u = -\frac{\pi}{2}+k2\pi \\
\\
\cos u = 0 & \Rightarrow u=\frac{\pi}{2}+k\pi \\
\cos u = 1 & \Rightarrow u=k2\pi \\
\cos u = -1 & \Rightarrow u = \pi +k2\pi \\
\end{split}
$$